F_mu_ref_par/examples/stack/refinement.v
@@ -1,0 +1,521 @@
+From iris.proofmode Require Import invariants ghost_ownership tactics.
+From iris.program_logic Require Import auth namespaces.
+From iris_logrel.F_mu_ref_par Require Import lang examples.lock
+     examples.stack.CG_stack examples.stack.FG_stack examples.stack.stack_rules
+     typing logrel_binary fundamental_binary rules_binary rules.
+Import uPred.
+
+Section Stack_refinement.
+  Context {Σ : gFunctors} {iS : cfgSG Σ} {iI : heapIG Σ}
+          {iSTK : authG lang Σ stackR}.
+
+  Ltac prove_disj N n n' :=
+    let Hneq := fresh "Hneq" in
+    let Hdsj := fresh "Hdsj" in
+    assert (Hneq : n ≠ n') by omega;
+    set (Hdsj := ndot_ne_disjoint N n n' Hneq); set_solver_ndisj.
+
+  Lemma FG_CG_counter_refinement N Δ
+        {HΔ : context_interp_Persistent Δ}
+    :
+      (@bin_log_related _ _ _ N Δ [] FG_stack CG_stack
+                        (TForall
+                           (TProd
+                              (TProd
+                                 (TArrow (TVar 0) TUnit)
+                                 (TArrow TUnit (TSum TUnit (TVar 0)))
+                              )
+                              (TArrow (TArrow (TVar 0) TUnit) TUnit)
+                        )) HΔ).
+  Proof.
+    (* executing the preambles *)
+    intros vs Hlen. destruct vs; [|inversion Hlen].
+    cbn -[FG_stack CG_stack].
+    intros ρ j K. iIntros "[#Hheap [#Hspec [_ Hj]]]".
+    rewrite ?empty_env_subst.
+    unfold CG_stack, FG_stack.
+    iApply wp_value; eauto.
+    iExists (TLamV _); iFrame "Hj".
+    iExists (_, _); iSplit; eauto.
+    iIntros {τi}. destruct τi as [τi Hτ]; simpl.
+    iAlways. iNext. clear j K. iIntros {j K} "Hj".
+    iPvs (steps_newlock _ _ _ j (K ++ [AppRCtx (LamV _)]) _ with "[Hj]")
+      as {l} "[Hj Hl]"; eauto.
+    rewrite fill_app; simpl.
+    iFrame "Hspec Hj"; trivial.
+    rewrite fill_app; simpl.
+    iPvs (step_lam _ _ _ j K _ _ _ _ with "[Hj]") as "Hj"; eauto.
+    iFrame "Hspec Hj"; trivial. simpl.
+    rewrite CG_locked_push_subst CG_locked_pop_subst
+            CG_iter_subst CG_snap_subst. simpl. asimpl.
+    iPvs (step_alloc _ _ _ j (K ++ [AppRCtx (LamV _)]) _ _ _ _ with "[Hj]")
+      as {stk'} "[Hj Hstk']"; eauto.
+    rewrite fill_app; simpl.
+    iFrame "Hspec Hj"; trivial.
+    rewrite fill_app; simpl.
+    iPvs (step_lam _ _ _ j K _ _ _ _ with "[Hj]") as "Hj"; eauto.
+    iFrame "Hspec Hj"; trivial. simpl.
+    rewrite CG_locked_push_subst CG_locked_pop_subst
+            CG_iter_subst CG_snap_subst. simpl. asimpl.
+    Unshelve.
+    all: try match goal with |- to_val _ = _ => auto using to_of_val end.
+    all: trivial.
+    iApply (@wp_bind _ _ _ [AppRCtx (LamV _); AllocCtx; FoldCtx]);
+      iApply wp_wand_l; iSplitR; [iIntros {v} "Hv"; iExact "Hv"|].
+    iApply wp_alloc; trivial; iFrame "Hheap"; iNext; iIntros {istk} "Histk".
+    iApply (@wp_bind _ _ _ [AppRCtx (LamV _)]);
+      iApply wp_wand_l; iSplitR; [iIntros {v} "Hv"; iExact "Hv"|].
+    iApply wp_alloc; trivial; iFrame "Hheap"; iNext; iIntros {stk} "Hstk".
+    simpl. iApply wp_lam; trivial. iNext. simpl.
+    rewrite FG_push_subst FG_pop_subst FG_iter_subst. simpl. asimpl.
+    (* establishing the invariant *)
+    iPvs (own_alloc (● (∅ : stackR))) as "Hemp".
+    { constructor; eauto. eapply cmra_unit_valid. }
+    iDestruct "Hemp" as {γ} "Hemp".
+    set (istkG := StackG _ _ γ).
+    change γ with (@stack_name _ istkG).
+    change iSTK with (@stack_inG _ istkG).
+    clearbody istkG. clear γ.
+    iAssert (@stack_owns _ istkG _ ∅) as "Hoe" with "[Hemp]".
+    { unfold stack_owns; rewrite big_sepM_empty; iFrame "Hemp"; trivial. }
+    iPvs (stack_owns_alloc ⊤ _ _ _ with "[Hoe Histk]") as "[Hoe Hls]".
+    { by iFrame "Hoe Histk". }
+    iAssert (StackLink τi (LocV istk, FoldV (InjLV UnitV)))
+      as "HLK" with "[Hls]".
+    { rewrite StackLink_unfold.
+      iExists _, _. iSplitR; simpl; trivial.
+      iFrame "Hls". iLeft. iSplit; trivial.
+    }
+    iAssert ((∃ istk v h, (stack_owns h)
+                         ★ stk' ↦ₛ v
+                         ★ stk ↦ᵢ (FoldV (LocV istk))
+                         ★ StackLink τi (LocV istk, v)
+                         ★ l ↦ₛ (♭v false)
+             )%I) as "Hinv" with "[Hoe Hstk Hstk' HLK Hl]".
+    { iExists _, _, _. by iFrame "Hoe Hstk' Hstk Hl HLK". }
+    iPvs (inv_alloc (N .@ 4) with "[Hinv]") as "#Hinv"; trivial.
+    { iNext; iExact "Hinv". }
+    clear istk.
+    Opaque stack_owns.
+    (* splitting *)
+    iApply wp_value; simpl; trivial.
+    iExists (PairV (PairV (CG_locked_pushV _ _) (CG_locked_popV _ _)) (LamV _)).
+    simpl. rewrite CG_locked_push_of_val CG_locked_pop_of_val. iFrame "Hj".
+    iExists (_, _), (_, _); iSplit; eauto.
+    iSplit.
+    (* refinement of push and pop *)
+    - iExists (_, _), (_, _); iSplit; eauto. iSplit.
+      + (* refinement of push *)
+        iAlways. clear j K. iIntros {j K v}. destruct v as [v1 v2].
+        iIntros "[#Hrel Hj]". simpl.
+        rewrite -(FG_push_folding (Loc stk)).
+        iLöb as "Hlat".
+        rewrite -> (FG_push_folding (Loc stk)) at 2.
+        iApply wp_lam; auto using to_of_val.
+        iNext.
+        rewrite -(FG_push_folding (Loc stk)).
+        asimpl.
+        iApply (@wp_bind _ _ _ [AppRCtx (LamV _)]);
+          iApply wp_wand_l; iSplitR; [iIntros {v} "Hv"; iExact "Hv"|].
+        iInv (N .@4) as {istk v h} "[Hoe [Hstk' [Hstk [HLK Hl]]]]".
+        iApply (wp_load _ _ _ _ _ _ _). iFrame "Hheap Hstk".
+        iNext. iIntros "Hstk".
+        iSplitL "Hoe Hstk' HLK Hl Hstk".
+        iNext. iExists _, _, _; by iFrame "Hoe Hstk' HLK Hl Hstk".
+        clear v h.
+        iApply wp_lam; auto using to_of_val.
+        iNext. asimpl.
+        iApply (@wp_bind _ _ _ [IfCtx _ _; CasRCtx (LocV _) (FoldV (LocV _));
+                                FoldCtx]);
+          iApply wp_wand_l; iSplitR; [iIntros {w} "Hw"; iExact "Hw"|].
+        iApply wp_alloc; simpl; trivial; [by rewrite to_of_val|].
+        iFrame "Hheap". iNext. iIntros {ltmp} "Hltmp".
+        iApply (@wp_bind _ _ _ [IfCtx _ _]);
+          iApply wp_wand_l; iSplitR; [iIntros {w} "Hw"; iExact "Hw"|].
+        iInv (N .@4) as {istk2 v h} "[Hoe [Hstk' [Hstk [HLK Hl]]]]".
+        (* deciding whether CAS will succeed or fail *)
+        destruct (decide (istk = istk2)) as [|Hneq]; subst.
+        * (* CAS succeeds *)
+          (* In this case, the specification pushes *)
+          iTimeless "Hstk'". iTimeless "Hl".
+          iPvs (steps_CG_locked_push _ _ _ j K _ _ _ _ _ with "[Hj Hl Hstk']")
+            as "[Hj [Hstk' Hl]]".
+          { rewrite CG_locked_push_of_val. by iFrame "Hspec Hstk' Hj". }
+          iApply wp_pvs.
+          iApply (wp_cas_suc _ _ _ _ _ _ _ _ _ _ _); simpl; trivial.
+          iFrame "Hheap Hstk". iNext. iIntros "Hstk".
+          iSplitR "Hj".
+          { iPvs (stack_owns_alloc with "[Hoe Hltmp]") as "[Hoe Hpt]".
+            { by iFrame "Hoe". }
+            iPvsIntro. iNext. iExists ltmp, _, _.
+            iFrame "Hoe Hstk' Hstk Hl".
+            do 2 rewrite StackLink_unfold.
+            rewrite -StackLink_unfold.
+            iExists _, _. iSplit; trivial.
+            iFrame "Hpt". iRight. iExists _, _, _, _.
+            repeat iSplitR; trivial.
+            iNext; trivial.
+          }
+          iPvsIntro.
+          iApply wp_if_true. iNext; iApply wp_value; trivial.
+          iExists UnitV. iFrame "Hj"; by iSplit.
+        * iApply (wp_cas_fail _ _ _ _ _ _ _ _ _ _ _ _ _ _); simpl; trivial.
+          iFrame "Hheap Hstk". iNext. iIntros "Hstk".
+          iSplitR "Hj".
+          { iNext. iExists _, _, _. by iFrame "Hoe Hstk' Hstk Hl". }
+          iApply wp_if_false. iNext. iApply "Hlat". by iNext.
+      + (* refinement of pop *)
+        iAlways. clear j K. iIntros {j K v}. destruct v as [v1 v2].
+        iIntros "[#Hrel Hj]". simpl.
+        iTimeless "Hrel". iDestruct "Hrel" as "[% %]". subst.
+        rewrite -(FG_pop_folding (Loc stk)).
+        iLöb as "Hlat".
+        rewrite -> (FG_pop_folding (Loc stk)) at 2.
+        iApply wp_lam; auto using to_of_val.
+        iNext.
+        rewrite -(FG_pop_folding (Loc stk)).
+        asimpl.
+        iApply (@wp_bind _ _ _ [AppRCtx (LamV _); UnfoldCtx]);
+          iApply wp_wand_l; iSplitR; [iIntros {v} "Hv"; iExact "Hv"|].
+        iInv (N .@4) as {istk v h} "[Hoe [Hstk' [Hstk [HLK Hl]]]]".
+        iApply wp_pvs.
+        iApply (wp_load _ _ _ _ _ _ _). iFrame "Hheap Hstk".
+        iNext. iIntros "Hstk".
+        (* Checking whether the stack is empty *)
+        iDestruct (StackLink_dup with "[HLK]") as "[HLK HLK']"; trivial.
+        rewrite -> StackLink_unfold at 2.
+        iDestruct "HLK'" as {istk2 w} "[HH [Hmpt HLK']]".
+        iDestruct "HH" as %HH. inversion HH; simpl in *; subst.
+        iDestruct "HLK'" as "[[% %]|HLK']".
+        * (* The stack is empty *)
+          simpl in *; subst.
+          iPvs (steps_CG_locked_pop_fail _ _ _ _ _ _ _ _ with "[Hj Hstk' Hl]")
+            as "[Hj [Hstk' Hl]]".
+          { by iFrame "Hspec Hstk' Hl Hj". }
+          iPvsIntro.
+          iSplitR "Hj Hmpt".
+          { iNext. iExists _, _, _. by iFrame "Hoe Hstk' Hstk Hl". }
+          iApply (@wp_bind _ _ _ [AppRCtx (LamV _)]);
+          iApply wp_wand_l; iSplitR; [iIntros {w} "Hw"; iExact "Hw"|].
+          iApply wp_Fold; simpl; auto using to_of_val.
+          iNext. iApply wp_lam; auto using to_of_val. iNext. asimpl.
+          clear h.
+          iApply (@wp_bind _ _ _ [AppRCtx (LamV _)]);
+          iApply wp_wand_l; iSplitR; [iIntros {w} "Hw"; iExact "Hw"|].
+          iInv (N .@4) as {istk3 w h} "[Hoe [Hstk' [Hstk [HLK Hl]]]]".
+          iDestruct (stack_owns_later_open_close with "[Hmpt Hoe]")
+            as "[Histk HLoe]".
+          { by iFrame "Hmpt". }
+          iApply (wp_load _ _ _ _ _ _ _). iFrame "Hheap Histk".
+          iNext. iIntros "Histk".
+          iSplitR "Hj".
+          { iNext. iExists _, _, _. iFrame "Hstk' Hstk HLK Hl".
+            iDestruct ("HLoe" with "[Histk]") as "[Hh _]"; trivial.
+          }
+          iApply wp_lam; simpl; trivial.
+          iNext. asimpl.
+          iApply wp_case_inl; trivial.
+          iNext. iApply wp_value; simpl; trivial. iExists (InjLV UnitV).
+          iSplit; trivial. iLeft. iExists (_, _); repeat iSplit; simpl; trivial.
+        * (* The stack is not empty *)
+          iPvsIntro. iSplitR "Hj Hmpt HLK'".
+          { iNext. iExists _, _, _. by iFrame "Hstk' Hstk HLK Hl". }
+          iApply (@wp_bind _ _ _ [AppRCtx (LamV _)]);
+          iApply wp_wand_l; iSplitR; [iIntros {w'} "Hw"; iExact "Hw"|].
+          iApply wp_Fold; simpl; auto using to_of_val.
+          iNext. iApply wp_lam; auto using to_of_val. iNext. asimpl.
+          clear h.
+          iApply (@wp_bind _ _ _ [AppRCtx (LamV _)]);
+          iApply wp_wand_l; iSplitR; [iIntros {w'} "Hw"; iExact "Hw"|].
+          iInv (N .@4) as {istk3 w' h} "[Hoe [Hstk' [Hstk [HLK Hl]]]]".
+          iDestruct (stack_owns_later_open_close with "[Hmpt Hoe]")
+            as "[Histk HLoe]".
+          { by iFrame "Hmpt". }
+          iApply (wp_load _ _ _ _ _ _ _). iFrame "Hheap Histk".
+          iNext. iIntros "Histk".
+          iDestruct ("HLoe" with "[Histk]") as "[Hh Hmpt]"; trivial.
+          iSplitR "Hj Hmpt HLK'".
+          { iNext. iExists _, _, _. by iFrame "Hstk' Hstk HLK Hl". }
+          iApply wp_lam; auto using to_of_val.
+          iNext. asimpl.
+          iDestruct "HLK'" as {y1 z1 y2 z2} "[% HLK']". subst. simpl.
+          iApply wp_case_inr; [simpl; by rewrite ?to_of_val |].
+          iNext.
+          iApply (@wp_bind _ _ _ [IfCtx _ _; CasRCtx (LocV _) (FoldV (LocV _))]);
+            iApply wp_wand_l; iSplitR; [iIntros {w} "Hw"; iExact "Hw"|].
+          asimpl. iApply wp_snd; [simpl; by rewrite ?to_of_val |
+                                  simpl; by rewrite ?to_of_val |].
+          simpl. iNext.
+          iApply (@wp_bind _ _ _ [IfCtx _ _]);
+            iApply wp_wand_l; iSplitR; [iIntros {w} "Hw"; iExact "Hw"|].
+          clear istk3 h. asimpl.
+          iInv (N .@4) as {istk3 w h} "[Hoe [Hstk' [Hstk [HLK Hl]]]]".
+          { by simpl; rewrite ?to_of_val; simpl. }
+          (* deciding whether CAS will succeed or fail *)
+          destruct (decide (istk2 = istk3)) as [|Hneq]; subst.
+          -- (* CAS succeeds *)
+            (* In this case, the specification pushes *)
+            iApply wp_pvs.
+            iApply (wp_cas_suc _ _ _ _ _ _ _ _ _ _ _).
+            iFrame "Hheap Hstk". iNext. iIntros "Hstk".
+            iClear "HLK'".
+            iDestruct (StackLink_dup with "[HLK]") as "[HLK HLK']"; trivial.
+            rewrite -> StackLink_unfold at 2.
+            iDestruct "HLK'" as {istk4 w2} "[HH [Hmpt' HLK']]".
+            iDestruct "HH" as %HH'. inversion HH'; simpl in *; subst.
+            iDestruct (stack_mapstos_agree with "[Hmpt Hmpt']")
+              as "[Hmpt [Hmpt' %]]".
+            { by iFrame "Hmpt Hmpt'". }
+            subst.
+            iDestruct "HLK'" as "[[Heq1 Heq2]|HLK']".
+            ++ iDestruct "Heq1" as %Heq1. inversion Heq1.
+            ++ iDestruct "HLK'" as {yn1 yn2 zn1 zn2}
+                                     "[Heq1 [Heq2 [#Hrel HLK'']]]".
+               iDestruct "Heq1" as %Heq1. iDestruct "Heq2" as %Heq2.
+               inversion Heq1; subst.
+               (* Now we have proven that specification can also pop. *)
+               rewrite CG_locked_pop_of_val.
+               iPvs (steps_CG_locked_pop_suc _ _ _ _ _ _ _ _ _ _
+                     with "[Hj Hstk' Hl]") as "[Hj [Hstk' Hl]]".
+               { by iFrame "Hspec Hstk' Hl Hj". }
+               iPvsIntro. iSplitR "Hj".
+               { iNext.
+                 iClear "Hmpt Hmpt' HLK". rewrite StackLink_unfold.
+                 iDestruct "HLK''" as {istk5 w2} "[% [Hmpt HLK]]".
+                 simpl in *; subst.
+                 iExists istk5, _, _. iFrame "Hoe Hstk' Hstk Hl".
+                 rewrite StackLink_unfold.
+                 iExists _, _; iSplitR; trivial.
+                 by iFrame "HLK".
+               }
+               iApply wp_if_true. iNext.
+               iApply (@wp_bind _ _ _ [InjRCtx]); iApply wp_wand_l;
+                 iSplitR; [iIntros {w} "Hw"; iExact "Hw"|].
+               iApply wp_fst; [simpl; by rewrite ?to_of_val |
+                               simpl; by rewrite ?to_of_val |].
+               iNext. iApply wp_value; simpl.
+               { by rewrite to_of_val. }
+               iExists (InjRV _); iFrame "Hj".
+               iRight. iExists (_, _). iSplit; trivial.
+          -- (* CAS will fail *)
+            iApply (wp_cas_fail _ _ _ _ _ _ _ _ _ _ _ _ _ _).
+            iFrame "Hheap Hstk". iNext. iIntros "Hstk".
+            iSplitR "Hj".
+            { iNext. iExists _, _, _. by iFrame "Hoe Hstk' Hstk HLK Hl". }
+            iApply wp_if_false. iNext. iApply "Hlat". by iNext.
+    - (* refinement of iter *)
+      iAlways. clear j K. iIntros {j K f}. destruct f as [f1 f2]. simpl.
+      rewrite -always_later. iIntros "[#Hfs Hj]".
+      iApply wp_lam; auto using to_of_val. iNext.
+      iPvs (step_lam _ _ _ _ _ _ _ _ _ _ with "[Hj]") as "Hj".
+      { by iFrame "Hspec Hj". }
+      asimpl. rewrite FG_iter_subst CG_snap_subst CG_iter_subst. asimpl.
+      replace (FG_iter (# f1)) with (# (FG_iterV (# f1)))
+        by (by rewrite FG_iter_of_val).
+      replace (CG_iter (# f2)) with (# (CG_iterV (# f2)))
+        by (by rewrite CG_iter_of_val).
+      iApply (@wp_bind _ _ _ [AppRCtx _]); iApply wp_wand_l;
+        iSplitR; [iIntros {w} "Hw"; iExact "Hw"|].
+      iInv (N .@4) as {istk3 w h} "[Hoe [Hstk' [Hstk [HLK Hl]]]]".
+      (* coarse-grained stack takes a snapshot *)
+      iTimeless "Hstk'"; iTimeless "Hl".
+      iPvs (steps_CG_snap _ _ _ _ (K ++ [AppRCtx _]) _ _ _ _
+            with "[Hstk' Hj Hl]") as "[Hj [Hstk' Hl]]".
+      { rewrite ?fill_app. simpl. by iFrame "Hspec Hstk' Hl Hj". }
+      iApply (wp_load _ _ _ _ _ _ _).
+      iFrame "Hheap Hstk". iNext. iIntros "Hstk".
+      iDestruct (StackLink_dup with "HLK") as "[HLK HLK']".
+      iSplitR "Hj HLK'".
+      { iNext. iExists _, _, _; by iFrame "Hoe Hstk' Hstk HLK Hl". }
+      clear h.
+      rewrite ?fill_app. simpl.
+      rewrite -FG_iter_folding.
+      iRevert {istk3 w} "Hj HLK'". iLöb as "Hlat".
+      iIntros {istk3 w} "Hj". iIntros "HLK". (* A bug in iIntros? *)
+      rewrite -> FG_iter_folding at 1.
+      iApply wp_lam; simpl; trivial.
+      rewrite -FG_iter_folding. asimpl. rewrite FG_iter_subst.
+      iNext.
+      iApply (@wp_bind _ _ _ [CaseCtx _ _; LoadCtx]); iApply wp_wand_l;
+        iSplitR; [iIntros {v} "Hw"; iExact "Hw"|].
+      iApply wp_Fold; simpl; trivial.
+      iNext. simpl.
+      iApply (@wp_bind _ _ _ [CaseCtx _ _]); iApply wp_wand_l;
+        iSplitR; [iIntros {v} "Hw"; iExact "Hw"|].
+      rewrite -> StackLink_unfold at 1.
+      iDestruct "HLK" as {istk4 v} "[Heq [Hmpt HLK']]".
+      iDestruct "Heq" as %Heq. inversion Heq; subst.
+      iInv (N .@4) as {istk5 v' h} "[Hoe [Hstk' [Hstk [HLK Hl]]]]".
+      iDestruct (stack_owns_later_open_close with "[Hmpt Hoe]")
+            as "[Histk HLoe]".
+      { by iFrame "Hmpt". }
+      iApply wp_pvs.
+      iApply (wp_load _ _ _ _ _ _ _). iFrame "Hheap Histk".
+      iNext. iIntros "Histk".
+      iDestruct ("HLoe" with "[Histk]") as "[Hh Hmpt]"; trivial.
+      iDestruct "HLK'" as "[[Heq1 Heq2]|HLK']".
+      * iDestruct "Heq1" as %Heq1. inversion Heq1.
+        iDestruct "Heq2" as %Heq2. inversion Heq2.
+        rewrite CG_iter_of_val.
+        iPvs (steps_CG_iter_end _ _ _ _ _ _ _ with "[Hj]") as "Hj".
+        { by iFrame "Hspec Hj". }
+        iPvsIntro. iSplitR "Hj".
+        { iNext. iExists _, _, _. by iFrame "Hh Hstk' Hstk HLK". }
+        iApply wp_case_inl; trivial.
+        iNext. iApply wp_value; trivial. iExists UnitV. iSplitL; trivial.
+          by iSplit.
+      * iDestruct "HLK'" as {yn1 yn2 zn1 zn2}
+                              "[Heq1 [Heq2 [#Hrel HLK'']]]".
+        iDestruct "Heq1" as %Heq1. inversion Heq1.
+        iDestruct "Heq2" as %Heq2. inversion Heq2.
+        rewrite CG_iter_of_val.
+        iPvs (steps_CG_iter _ _ _ _ _ _ _ _ _ with "[Hj]") as "Hj".
+        { by iFrame "Hspec Hj". }
+        iPvsIntro. iSplitR "Hj HLK''".
+        { iNext. iExists _, _, _. by iFrame "Hh Hstk' Hstk HLK". }
+        simpl.
+        iApply wp_case_inr; simpl; rewrite ?to_of_val; trivial.
+        rewrite FG_iter_subst CG_iter_subst. asimpl.
+        iNext.
+        iApply (@wp_bind _ _ _ [AppRCtx (LamV _); AppRCtx _]);
+          iApply wp_wand_l; iSplitR; [iIntros {w'} "Hw"; iExact "Hw"|].
+        iApply wp_fst; simpl; rewrite ?to_of_val; trivial. iNext.
+        iApply (@wp_bind _ _ _ [AppRCtx (LamV _)]);
+          iApply wp_wand_l; iSplitR; [iIntros {w'} "Hw"; iExact "Hw"|].
+        rewrite -> StackLink_unfold at 1.
+        iDestruct "HLK''" as {istk6 w'} "[% HLK]".
+        simpl in *; subst.
+        iSpecialize ("Hfs" $! _ (K ++ [AppRCtx (LamV _)]) (yn1, zn1)).
+        rewrite fill_app; simpl.
+        iApply wp_wand_l; iSplitR "Hj"; [|iApply "Hfs"; by iFrame "Hrel Hj"].
+        iIntros {u}; simpl.
+        iIntros "Hj". iDestruct "Hj" as {z} "[Hj [% %]]".
+        rewrite fill_app; simpl. subst. asimpl.
+        iPvs (step_lam _ _ _ _ _ _ _ _ _ _ with "[Hj]") as "Hj".
+        { by iFrame "Hspec Hj". } asimpl. rewrite CG_iter_subst. asimpl.
+        replace (CG_iter (# f2)) with (# (CG_iterV (# f2)))
+          by (by rewrite CG_iter_of_val).
+        iPvs (step_snd _ _ _ _ (K ++ [AppRCtx _]) _ _ _ _ _ _ _ with "[Hj]")
+          as "Hj".
+        { rewrite fill_app; simpl. by iFrame "Hspec Hj". }
+        rewrite fill_app; simpl.
+        iApply wp_lam; simpl; trivial.
+        iNext. rewrite FG_iter_subst. asimpl.
+        replace (FG_iter (# f1)) with (# (FG_iterV (# f1)))
+          by (by rewrite FG_iter_of_val).
+        iApply (@wp_bind _ _ _ [AppRCtx _]);
+          iApply wp_wand_l; iSplitR; [iIntros {w''} "Hw"; iExact "Hw"|].
+        iApply (wp_snd _ _ _ _ _ _); auto using to_of_val.
+        simpl. iNext. rewrite -FG_iter_folding.
+        iSpecialize ("Hlat" $! istk6 zn2).
+        iApply ("Hlat" with "[Hj] [HLK]"); trivial.
+        rewrite -> StackLink_unfold at 2.
+        iExists _, _; iSplitR; trivial.
+        Unshelve.
+        all: try match goal with
+                   |- to_val _ = _ => simpl; by rewrite ?to_of_val
+                 end.
+        all: trivial.
+        all: try match goal with
+                   |- _ ≠ _ => let H := fresh "H" in intros H; inversion H; auto
+                 end.
+        (* This seems to be a bug in all: mechanism!? *)
+        match goal with
+          |- @subseteq
+              _ _ (nclose (N .@ ?A))
+              (@difference _ _ ⊤ (nclose (N .@ ?B))) =>
+          abstract (prove_disj N A B)
+        end.
+        match goal with
+          |- @subseteq
+              _ _ (nclose (N .@ ?A))
+              (@difference _ _ ⊤ (nclose (N .@ ?B))) =>
+          abstract (prove_disj N A B)
+        end.
+        match goal with
+          |- @subseteq
+              _ _ (nclose (N .@ ?A))
+              (@difference _ _ ⊤ (nclose (N .@ ?B))) =>
+          abstract (prove_disj N A B)
+        end.
+        match goal with
+          |- @subseteq
+              _ _ (nclose (N .@ ?A))
+              (@difference _ _ ⊤ (nclose (N .@ ?B))) =>
+          abstract (prove_disj N A B)
+        end.
+        match goal with
+          |- @subseteq
+              _ _ (nclose (N .@ ?A))
+              (@difference _ _ ⊤ (nclose (N .@ ?B))) =>
+          abstract (prove_disj N A B)
+        end.
+        match goal with
+          |- @subseteq
+              _ _ (nclose (N .@ ?A))
+              (@difference _ _ ⊤ (nclose (N .@ ?B))) =>
+          abstract (prove_disj N A B)
+        end.
+        match goal with
+          |- @subseteq
+              _ _ (nclose (N .@ ?A))
+              (@difference _ _ ⊤ (nclose (N .@ ?B))) =>
+          abstract (prove_disj N A B)
+        end.
+        match goal with
+          |- @subseteq
+              _ _ (nclose (N .@ ?A))
+              (@difference _ _ ⊤ (nclose (N .@ ?B))) =>
+          abstract (prove_disj N A B)
+        end.
+        match goal with
+          |- @subseteq
+              _ _ (nclose (N .@ ?A))
+              (@difference _ _ ⊤ (nclose (N .@ ?B))) =>
+          abstract (prove_disj N A B)
+        end.
+        match goal with
+          |- @subseteq
+              _ _ (nclose (N .@ ?A))
+              (@difference _ _ ⊤ (nclose (N .@ ?B))) =>
+          abstract (prove_disj N A B)
+        end.
+        match goal with
+          |- @subseteq
+              _ _ (nclose (N .@ ?A))
+              (@difference _ _ ⊤ (nclose (N .@ ?B))) =>
+          abstract (prove_disj N A B)
+        end.
+        match goal with
+          |- @subseteq
+              _ _ (nclose (N .@ ?A))
+              (@difference _ _ ⊤ (nclose (N .@ ?B))) =>
+          abstract (prove_disj N A B)
+        end.
+        match goal with
+          |- @subseteq
+              _ _ (nclose (N .@ ?A))
+              (@difference _ _ ⊤ (nclose (N .@ ?B))) =>
+          abstract (prove_disj N A B)
+        end.
+        match goal with
+          |- @subseteq
+              _ _ (nclose (N .@ ?A))
+              (@difference _ _ ⊤ (nclose (N .@ ?B))) =>
+          abstract (prove_disj N A B)
+        end.
+        match goal with
+          |- @subseteq
+              _ _ (nclose (N .@ ?A))
+              (@difference _ _ ⊤ (nclose (N .@ ?B))) =>
+          abstract (prove_disj N A B)
+        end.
+        match goal with
+          |- @subseteq
+              _ _ (nclose (N .@ ?A))
+              (@difference _ _ ⊤ (nclose (N .@ ?B))) =>
+          abstract (prove_disj N A B)
+        end.
+  Qed.
+
+End Stack_refinement.
